Mica/Base.lean
@@ -2,3 +2,4 @@
 
 import Mica.Base.Fresh
 import Mica.Base.Except
+import Mica.Base.Fixpoint
